chore: split LTS/Basic.lean into more manageable pieces (#453)
This PR splits `Cslib/Foundations/Semantics/LTS/Basic.lean` into 7 files
with the following dependencies among them:
- Basic.lean
- Execution.lean, which imports Basic.lean
- OmegaExecution.lean, which imports Execution.lean
- Total.lean, which imports OmegaExecution.lean
- HasTau.lean, which imports Basic.lean
- Divergence.lean, which imports HasTau.lean and OmegaExecution.lean
- Union.lean, which imports Basic.lean

Other files which formerly import LTS/Basic.lean now import only the
"lowest" necessary file in the above hierarchy. LTS/Basic.lean now
imports only Cslib.Init and some mathlib files.

I also took the opportunity to rename a few theorems to more rational
and systematic names.

---------

Co-authored-by: Chris Henson <chrishenson.net@gmail.com>

Cslib/Foundations/Semantics/LTS/Basic.lean
@@ -6,8 +6,9 @@ Authors: Fabrizio Montesi
 
 module
 
-public import Cslib.Foundations.Data.OmegaSequence.Flatten
-public import Cslib.Foundations.Semantics.FLTS.Basic
+public import Cslib.Init
+public import Mathlib.Data.Set.Finite.Basic
+public import Mathlib.Order.SetNotation
 
 @[expose] public section
 
@@ -59,14 +60,7 @@ structure LTS (State : Type u) (Label : Type v) where
   /-- The transition relation. -/
   Tr : State → Label → State → Prop
 
-/-- Returns the relation that relates all states `s1` and `s2` via a fixed transition label `μ`. -/
-def LTS.Tr.toRelation (lts : LTS State Label) (μ : Label) : State → State → Prop :=
-  fun s1 s2 => lts.Tr s1 μ s2
-
-/-- Any homogeneous relation can be seen as an LTS where all transitions have the same label. -/
-def Relation.toLTS [DecidableEq Label] (r : State → State → Prop) (μ : Label) :
-  LTS State Label where
-  Tr := fun s1 μ' s2 => if μ' = μ then r s1 s2 else False
+namespace LTS
 
 section MultiStep
 
@@ -85,7 +79,7 @@ rule. This makes working with lists of labels more convenient, because we follow
 construction. It is also similar to what is done in the `SimpleGraph` library in mathlib.)
 -/
 @[scoped grind]
-inductive LTS.MTr (lts : LTS State Label) : State → List Label → State → Prop where
+inductive MTr (lts : LTS State Label) : State → List Label → State → Prop where
   | refl {s : State} : lts.MTr s [] s
   | stepL {s1 : State} {μ : Label} {s2 : State} {μs : List Label} {s3 : State} :
     lts.Tr s1 μ s2 → lts.MTr s2 μs s3 →
@@ -93,40 +87,40 @@ inductive LTS.MTr (lts : LTS State Label) : State → List Label → State → P
 
 /-- Any transition is also a multistep transition. -/
 @[scoped grind →]
-theorem LTS.MTr.single {s1 : State} {μ : Label} {s2 : State} :
+theorem MTr.single {s1 : State} {μ : Label} {s2 : State} :
   lts.Tr s1 μ s2 → lts.MTr s1 [μ] s2 := by
   intro h
-  apply LTS.MTr.stepL
+  apply MTr.stepL
   · exact h
-  · apply LTS.MTr.refl
+  · apply MTr.refl
 
 /-- Any multistep transition can be extended by adding a transition. -/
-theorem LTS.MTr.stepR {s1 : State} {μs : List Label} {s2 : State} {μ : Label} {s3 : State} :
+theorem MTr.stepR {s1 : State} {μs : List Label} {s2 : State} {μ : Label} {s3 : State} :
   lts.MTr s1 μs s2 → lts.Tr s2 μ s3 → lts.MTr s1 (μs ++ [μ]) s3 := by
   intro h1 h2
   induction h1
-  case refl s1' => exact LTS.MTr.single lts h2
+  case refl s1' => exact MTr.single lts h2
   case stepL s1' μ' s2' μs' s3' h1' h3 ih =>
-    apply LTS.MTr.stepL
+    apply MTr.stepL
     · exact h1'
     · apply ih h2
 
 /-- Multistep transitions can be composed. -/
 @[scoped grind <=]
-theorem LTS.MTr.comp {s1 : State} {μs1 : List Label} {s2 : State} {μs2 : List Label} {s3 : State} :
+theorem MTr.comp {s1 : State} {μs1 : List Label} {s2 : State} {μs2 : List Label} {s3 : State} :
   lts.MTr s1 μs1 s2 → lts.MTr s2 μs2 s3 →
   lts.MTr s1 (μs1 ++ μs2) s3 := by
   intro h1 h2
   induction h1
   case refl => assumption
   case stepL s1 μ s' μs1' s'' h1' h3 ih  =>
-    apply LTS.MTr.stepL
+    apply MTr.stepL
     · exact h1'
     · apply ih h2
 
 /-- Any 1-sized multistep transition implies a transition with the same states and label. -/
 @[scoped grind .]
-theorem LTS.MTr.single_invert (s1 : State) (μ : Label) (s2 : State) :
+theorem MTr.single_invert (s1 : State) (μ : Label) (s2 : State) :
   lts.MTr s1 [μ] s2 → lts.Tr s1 μ s2 := by
   intro h
   cases h
@@ -136,467 +130,28 @@ theorem LTS.MTr.single_invert (s1 : State) (μ : Label) (s2 : State) :
 
 /-- In any zero-steps multistep transition, the origin and the derivative are the same. -/
 @[scoped grind .]
-theorem LTS.MTr.nil_eq (h : lts.MTr s1 [] s2) : s1 = s2 := by
+theorem MTr.nil_eq (h : lts.MTr s1 [] s2) : s1 = s2 := by
   cases h
   rfl
-
-/-- LTS.Execution extends LTS.MTr by providing the intermediate states of a multistep transition. -/
-@[scoped grind =]
-def LTS.Execution (lts : LTS State Label) (s1 : State) (μs : List Label) (s2 : State)
-    (ss : List State) : Prop :=
-  ∃ _ : ss.length = μs.length + 1, ss[0] = s1 ∧ ss[ss.length - 1] = s2 ∧
-  ∀ k, {_ : k < μs.length} → lts.Tr ss[k] μs[k] ss[k + 1]
-
-/-- Every execution has at least one intermediate state. -/
-@[scoped grind →]
-theorem LTS.execution_nonEmpty_states (h : lts.Execution s1 μs s2 ss) :
-    ss ≠ [] := by grind
-
-/-- Every state has an execution of zero steps terminating in itself. -/
-@[scoped grind ⇒]
-theorem LTS.Execution.refl (lts : LTS State Label) (s : State) : lts.Execution s [] s [s] := by
-  grind
-
-/-- Equivalent of `MTr.stepL` for executions. -/
-theorem LTS.Execution.stepL {lts : LTS State Label} (htr : lts.Tr s1 μ s2)
-    (hexec : lts.Execution s2 μs s3 ss) : lts.Execution s1 (μ :: μs) s3 (s1 :: ss) := by grind
-
-/-- Deconstruction of executions with `List.cons`. -/
-theorem LTS.execution_cons_invert (h : lts.Execution s1 (μ :: μs) s2 (s1 :: ss)) :
-    lts.Execution (ss[0]'(by grind)) μs s2 ss := by
-  obtain ⟨_, _, _, h4⟩ := h
-  exists (by grind)
-  constructorm* _∧_
-  · rfl
-  · grind
-  · intro k valid
-    specialize h4 k <;> grind
-
-open scoped LTS.Execution in
-/-- A multistep transition implies the existence of an execution. -/
-@[scoped grind →]
-theorem LTS.execution_of_mTr {lts : LTS State Label}
-    {s1 : State} {μs : List Label} {s2 : State}
-    (h : lts.MTr s1 μs s2) : ∃ ss : List State, lts.Execution s1 μs s2 ss := by
-  induction h
-  case refl t =>
-    use [t]
-    grind
-  case stepL t1 μ t2 μs t3 htr hmtr ih =>
-    obtain ⟨ss', _⟩ := ih
-    use t1 :: ss'
-    grind
-
-/-- Converts an execution into a multistep transition. -/
-@[scoped grind →]
-theorem LTS.mTr_of_execution (hexec : lts.Execution s1 μs s2 ss) :
-    lts.MTr s1 μs s2 := by
-  induction ss generalizing s1 μs
-  case nil => grind
-  case cons s1' ss ih =>
-    let ⟨hlen, hstart, hfinal, hexec'⟩ := hexec
-    have : s1' = s1 := by grind
-    rw [this] at hexec' hexec
-    cases μs
-    · grind
-    case cons μ μs =>
-      specialize ih (s1 := ss[0]'(by grind)) (μs := μs)
-      apply LTS.execution_cons_invert at hexec
-      apply LTS.MTr.stepL
-      · have : lts.Tr s1 μ (ss[0]'(by grind)) := by grind
-        apply this
-      · grind
-
-/-- Correspondence of multistep transitions and executions. -/
-@[scoped grind =]
-theorem LTS.mTr_iff_execution :
-    lts.MTr s1 μs s2 ↔ ∃ ss : List State, lts.Execution s1 μs s2 ss := by
-  grind
-
-private lemma LTS.Execution.comp_helper
-    {lts : LTS State Label} {s r t : State} {μs1 μs2 : List Label} {ss1 ss2 : List State}
-    (h1 : lts.Execution s μs1 r ss1) (h2 : lts.Execution r μs2 t ss2)
-    (k : ℕ) (h_k : k < ss2.length) :
-    (ss1 ++ ss2.tail)[μs1.length + k]'(by grind) = ss2[k] := by
-  by_cases h : k = 0
-  · simp (disch := grind) only [h, add_zero, List.getElem_append_left]
-    grind
-  · simp (disch := grind) only [List.getElem_append_right, List.getElem_tail]
-    have : μs1.length + k - ss1.length + 1 = k := by grind
-    grind
-
-/-- The composition of two executions is an execution. -/
-theorem LTS.Execution.comp
-    {lts : LTS State Label} {s r t : State} {μs1 μs2 : List Label} {ss1 ss2 : List State}
-    (h1 : lts.Execution s μs1 r ss1) (h2 : lts.Execution r μs2 t ss2) :
-    lts.Execution s (μs1 ++ μs2) t (ss1 ++ ss2.tail) := by
-  have h0 : (ss1 ++ ss2.tail).length = (μs1 ++ μs2).length + 1 := by grind
-  use h0
-  split_ands
-  · grind
-  · have := LTS.Execution.comp_helper h1 h2 μs2.length
-    grind only [Execution, = List.length_append]
-  · intro k h_k
-    by_cases k < μs1.length
-    · grind only [Execution, = List.getElem_append]
-    · have := LTS.Execution.comp_helper h1 h2 (k - μs1.length)
-      have := LTS.Execution.comp_helper h1 h2 (k - μs1.length + 1)
-      grind
-
-/-- An execution can be split at any intermediate state into two executions. -/
-theorem LTS.Execution.split
-    {lts : LTS State Label} {s t : State} {μs : List Label} {ss : List State}
-    (he : lts.Execution s μs t ss) (n : ℕ) (hn : n ≤ μs.length) :
-    lts.Execution s (μs.take n) (ss[n]'(by grind)) (ss.take (n + 1)) ∧
-    lts.Execution (ss[n]'(by grind)) (μs.drop n) t (ss.drop n) := by
-  have : n + (ss.length - n - 1) = ss.length - 1 := by grind
-  simp [Execution]
-  grind
-
-/-- A multistep transition over a concatenation can be split into two multistep transitions. -/
-theorem LTS.MTr.split {lts : LTS State Label} {s0 : State} {μs1 μs2 : List Label} {s2 : State}
-    (h : lts.MTr s0 (μs1 ++ μs2) s2) : ∃ s1, lts.MTr s0 μs1 s1 ∧ lts.MTr s1 μs2 s2 := by
-  obtain ⟨ss, h_ss⟩ := LTS.execution_of_mTr h
-  have := LTS.Execution.split h_ss μs1.length
-  grind
 
 /-- A state `s1` can reach a state `s2` if there exists a multistep transition from
 `s1` to `s2`. -/
 @[scoped grind =]
-def LTS.CanReach (s1 s2 : State) : Prop :=
+def CanReach (s1 s2 : State) : Prop :=
   ∃ μs, lts.MTr s1 μs s2
 
 /-- Any state can reach itself. -/
 @[scoped grind .]
-theorem LTS.CanReach.refl (s : State) : lts.CanReach s s := by
+theorem CanReach.refl (s : State) : lts.CanReach s s := by
   exists []
-  apply LTS.MTr.refl
+  apply MTr.refl
 
 /-- The LTS generated by a state `s` is the LTS given by all the states reachable from `s`. -/
 @[scoped grind =]
-def LTS.generatedBy (s : State) : LTS {s' : State // lts.CanReach s s'} Label where
+def generatedBy (s : State) : LTS {s' : State // lts.CanReach s s'} Label where
   Tr := fun s1 μ s2 => lts.CanReach s s1 ∧ lts.CanReach s s2 ∧ lts.Tr s1 μ s2
 
-/-- Returns the relation that relates all states `s1` and `s2` via a fixed list of transition
-labels `μs`. -/
-def LTS.MTr.toRelation (lts : LTS State Label) (μs : List Label) : State → State → Prop :=
-  fun s1 s2 => lts.MTr s1 μs s2
-
-/-! ### Calc tactic support for MTr -/
-
-/-- Transitions can be chained. -/
-instance (lts : LTS State Label) :
-  Trans
-    (LTS.Tr.toRelation lts μ1)
-    (LTS.Tr.toRelation lts μ2)
-    (LTS.MTr.toRelation lts [μ1, μ2]) where
-  trans := by
-    intro s1 s2 s3 htr1 htr2
-    apply LTS.MTr.single at htr1
-    apply LTS.MTr.single at htr2
-    apply LTS.MTr.comp lts htr1 htr2
-
-/-- Transitions can be chained with multi-step transitions. -/
-instance (lts : LTS State Label) :
-  Trans
-    (LTS.Tr.toRelation lts μ)
-    (LTS.MTr.toRelation lts μs)
-    (LTS.MTr.toRelation lts (μ :: μs)) where
-  trans := by
-    intro s1 s2 s3 htr1 hmtr2
-    apply LTS.MTr.single at htr1
-    apply LTS.MTr.comp lts htr1 hmtr2
-
-/-- Multi-step transitions can be chained with transitions. -/
-instance (lts : LTS State Label) :
-  Trans
-    (LTS.MTr.toRelation lts μs)
-    (LTS.Tr.toRelation lts μ)
-    (LTS.MTr.toRelation lts (μs ++ [μ])) where
-  trans := by
-    intro s1 s2 s3 hmtr1 htr2
-    apply LTS.MTr.single at htr2
-    apply LTS.MTr.comp lts hmtr1 htr2
-
-/-- Multi-step transitions can be chained. -/
-instance (lts : LTS State Label) :
-  Trans
-    (LTS.MTr.toRelation lts μs1)
-    (LTS.MTr.toRelation lts μs2)
-    (LTS.MTr.toRelation lts (μs1 ++ μs2)) where
-  trans := by
-    intro s1 s2 s3 hmtr1 hmtr2
-    apply LTS.MTr.comp lts hmtr1 hmtr2
-
 end MultiStep
-
-section ωMultiStep
-
-/-! ## Infinite sequences of transitions
--/
-
-/-- An infinite execution is conceptually an infinite sequence of transitions. But it is
-technically more convenient to separate the states and the labels into two ω-sequences. -/
-@[scoped grind]
-def LTS.OmegaExecution (lts : LTS State Label)
-    (ss : ωSequence State) (μs : ωSequence Label) : Prop :=
-  ∀ i, lts.Tr (ss i) (μs i) (ss (i + 1))
-
-variable {lts : LTS State Label}
-
-open ωSequence
-
-/-- Any finite execution extracted from an infinite execution is valid. -/
-theorem LTS.OmegaExecution.extract_execution
-    (h : lts.OmegaExecution ss μs) {n m : ℕ} (hnm : n ≤ m) :
-    lts.Execution (ss n) (μs.extract n m) (ss m) (ss.extract n (m + 1)) := by
-  grind
-
-/-- Any multistep transition extracted from an infinite execution is valid. -/
-theorem LTS.OmegaExecution.extract_mTr
-    (h : lts.OmegaExecution ss μs) {n m : ℕ} (hnm : n ≤ m) :
-    lts.MTr (ss n) (μs.extract n m) (ss m) := by
-  grind [LTS.OmegaExecution.extract_execution h hnm]
-
-/-- Prepends an infinite execution with a transition. -/
-theorem LTS.OmegaExecution.cons (htr : lts.Tr s μ t)
-    (hωtr : lts.OmegaExecution ss μs) (hm : ss 0 = t) :
-    lts.OmegaExecution (s ::ω ss) (μ ::ω μs) := by
-  intro i
-  induction i <;> grind
-
-/-- Prepends an infinite execution with a finite execution. -/
-theorem LTS.OmegaExecution.append
-    (hmtr : lts.MTr s μl t) (hωtr : lts.OmegaExecution ss μs) (hm : ss 0 = t) :
-    ∃ ss', lts.OmegaExecution ss' (μl ++ω μs) ∧
-      ss' 0 = s ∧ ss' μl.length = t ∧ ss'.drop μl.length = ss := by
-  obtain ⟨sl, _, _, _, _⟩ := LTS.execution_of_mTr hmtr
-  use sl.take μl.length ++ω ss
-  split_ands
-  · intro n
-    by_cases n < μl.length
-    · grind [get_append_left]
-    · by_cases n = μl.length
-      · grind [get_append_left, get_append_right']
-      · grind [get_append_right', hωtr (n - μl.length - 1)]
-  · grind [get_append_left]
-  · grind [get_append_left]
-  · grind [drop_append_of_ge_length]
-
-open Nat in
-/-- Concatenating an infinite sequence of finite executions. -/
-theorem LTS.OmegaExecution.flatten_execution [Inhabited Label]
-    {ts : ωSequence State} {μls : ωSequence (List Label)} {sls : ωSequence (List State)}
-    (hexec : ∀ k, lts.Execution (ts k) (μls k) (ts (k + 1)) (sls k))
-    (hpos : ∀ k, (μls k).length > 0) :
-    ∃ ss, lts.OmegaExecution ss μls.flatten ∧
-      ∀ k, ss.extract (μls.cumLen k) (μls.cumLen (k + 1)) = (sls k).take (μls k).length := by
-  have : Inhabited State := by exact {default := ts 0}
-  let segs := ωSequence.mk fun k ↦ (sls k).take (μls k).length
-  have h_len : μls.cumLen = segs.cumLen := by ext k; induction k <;> grind
-  have h_pos (k : ℕ) : (segs k).length > 0 := by grind [List.eq_nil_iff_length_eq_zero]
-  have h_mono := cumLen_strictMono h_pos
-  have h_zero := cumLen_zero (ls := segs)
-  have h_seg0 (k : ℕ) : (segs k)[0]! = ts k := by grind
-  use segs.flatten
-  split_ands
-  · intro n
-    simp only [h_len, flatten_def]
-    simp only [LTS.Execution] at hexec
-    have := segment_lower_bound h_mono h_zero n
-    by_cases h_n : n + 1 < segs.cumLen (segment segs.cumLen n + 1)
-    · have := segment_range_val h_mono (by grind) h_n
-      have : n + 1 - segs.cumLen (segment segs.cumLen n) < (μls (segment segs.cumLen n)).length :=
-        by grind
-      grind
-    · have h1 : segs.cumLen (segment segs.cumLen n + 1) = n + 1 := by
-        grind [segment_upper_bound h_mono h_zero n]
-      have h2 : segment segs.cumLen (n + 1) = segment segs.cumLen n + 1 := by
-        simp [← h1, segment_idem h_mono]
-      have : n + 1 - segs.cumLen (segment segs.cumLen n) = (μls (segment segs.cumLen n)).length :=
-        by grind
-      have h3 : ts (segment segs.cumLen n + 1) =
-          (sls (segment segs.cumLen n))[n + 1 - segs.cumLen (segment segs.cumLen n)]! := by
-        grind
-      simp [h1, h2, h_seg0, h3]
-      grind
-  · simp [h_len, extract_flatten h_pos, segs]
-
-/-- Concatenating an infinite sequence of multistep transitions. -/
-theorem LTS.OmegaExecution.flatten_mTr [Inhabited Label]
-    {ts : ωSequence State} {μls : ωSequence (List Label)}
-    (hmtr : ∀ k, lts.MTr (ts k) (μls k) (ts (k + 1))) (hpos : ∀ k, (μls k).length > 0) :
-    ∃ ss, lts.OmegaExecution ss μls.flatten ∧ ∀ k, ss (μls.cumLen k) = ts k := by
-  choose sls h_sls using fun k ↦ LTS.execution_of_mTr (hmtr k)
-  obtain ⟨ss, h_ss, h_seg⟩ := LTS.OmegaExecution.flatten_execution h_sls hpos
-  use ss, h_ss
-  intro k
-  have h1 : 0 < (ss.extract (μls.cumLen k) (μls.cumLen (k + 1))).length := by grind
-  grind [List.getElem_of_eq (h_seg k) h1]
-
-end ωMultiStep
-
-section Total
-
-/-! ## Total LTS -/
-
-open Sum ωSequence
-
-variable {State Label : Type*} {lts : LTS State Label}
-
-/-- An LTS is total iff every state has a `μ`-derivative for every label `μ`. -/
-class LTS.Total (lts : LTS State Label) where
-  /-- The condition of being total. -/
-  total s μ : ∃ s', lts.Tr s μ s'
-
-/-- Choose an FLTS that is a "sub-LTS" of a total LTS. -/
-noncomputable def LTS.chooseFLTS (lts : LTS State Label) [h : lts.Total] : FLTS State Label where
-  tr s μ := Classical.choose <| h.total s μ
-
-/-- The FLTS chosen by `LTS.chooseFLTS` always provides legal transitions. -/
-theorem LTS.chooseFLTS.total (lts : LTS State Label) [h : lts.Total] (s : State) (μ : Label) :
-    lts.Tr s μ (lts.chooseFLTS.tr s μ) :=
-  Classical.choose_spec <| h.total s μ
-
-/-- `LTS.chooseOmegaExecution` builds an infinite execution of a total LTS from any starting state
-and over any infinite sequence of labels. -/
-noncomputable def LTS.chooseOmegaExecution (lts : LTS State Label) [lts.Total]
-    (s : State) (μs : ωSequence Label) : ℕ → State
-  | 0 => s
-  | n + 1 => lts.chooseFLTS.tr (lts.chooseOmegaExecution s μs n) (μs n)
-
-/-- If a LTS is total, then there exists an infinite execution from any starting state and
-over any infinite sequence of labels. -/
-theorem LTS.Total.omegaExecution_exists [h : lts.Total] (s : State) (μs : ωSequence Label) :
-    ∃ ss, lts.OmegaExecution ss μs ∧ ss 0 = s := by
-  use lts.chooseOmegaExecution s μs
-  grind [LTS.chooseOmegaExecution, LTS.chooseFLTS.total]
-
-/-- If a LTS is total, then any finite execution can be extended to an infinite execution,
-provided that the label type is inbabited. -/
-theorem LTS.Total.mTr_omegaExecution [Inhabited Label] [ht : lts.Total]
-    {μl : List Label} {s t : State} (hm : lts.MTr s μl t) :
-    ∃ μs ss, lts.OmegaExecution ss (μl ++ω μs) ∧ ss 0 = s ∧ ss μl.length = t := by
-  let μs : ωSequence Label := .const default
-  obtain ⟨ss', ho, h0⟩ := LTS.Total.omegaExecution_exists (h := ht) t μs
-  grind [LTS.OmegaExecution.append hm ho h0]
-
-/-- `LTS.totalize` constructs a total LTS from any given LTS by adding a sink state. -/
-def LTS.totalize (lts : LTS State Label) : LTS (State ⊕ Unit) Label where
-  Tr s' μ t' := match s', t' with
-    | inl s, inl t => lts.Tr s μ t
-    | _, inr () => True
-    | inr (), inl _ => False
-
-/-- The LTS constructed by `LTS.totalize` is indeed total. -/
-instance (lts : LTS State Label) : lts.totalize.Total where
-  total _ _ := by simp [LTS.totalize]
-
-/-- In `LTS.totalize`, there is no finite execution from the sink state to any non-sink state. -/
-theorem LTS.totalize.not_right_left {μs : List Label} {t : State} :
-    ¬ lts.totalize.MTr (inr ()) μs (inl t) := by
-  intro h
-  generalize h_s : (inr () : State ⊕ Unit) = s'
-  generalize h_t : (inl t : State ⊕ Unit) = t'
-  rw [h_s, h_t] at h
-  induction h <;> grind [LTS.totalize]
-
-/-- In `LTS.totalize`, the transitions between non-sink states correspond exactly to
-the transitions in the original LTS. -/
-@[simp]
-theorem LTS.totalize.tr_left_iff {μ : Label} {s t : State} :
-    lts.totalize.Tr (inl s) μ (inl t) ↔ lts.Tr s μ t := by
-  simp [LTS.totalize]
-
-/-- In `LTS.totalize`, the multistep transitions between non-sink states correspond exactly to
-the multistep transitions in the original LTS. -/
-@[simp]
-theorem LTS.totalize.mtr_left_iff {μs : List Label} {s t : State} :
-    lts.totalize.MTr (inl s) μs (inl t) ↔ lts.MTr s μs t := by
-  constructor <;> intro h
-  · generalize h_s : (inl s : State ⊕ Unit) = s'
-    generalize h_t : (inl t : State ⊕ Unit) = t'
-    rw [h_s, h_t] at h
-    induction h generalizing s
-    case refl _ => grind [LTS.MTr]
-    case stepL t1' μ t2' μs t3' h_tr h_mtr h_ind =>
-      obtain ⟨rfl⟩ := h_s
-      cases t2'
-      case inl t2 => grind [LTS.MTr, totalize.tr_left_iff.mp h_tr]
-      case inr t2 => grind [totalize.not_right_left]
-  · induction h
-    case refl _ => grind [LTS.MTr]
-    case stepL t1 μ t2 μs t3 h_tr h_mtr h_ind =>
-      grind [LTS.MTr, totalize.tr_left_iff.mpr h_tr]
-
-end Total
-
-section Termination
-/-! ## Definitions about termination -/
-
-variable {State} {Label} (lts : LTS State Label) {Terminated : State → Prop}
-
-/-- A state 'may terminate' if it can reach a terminated state. The definition of `Terminated`
-is a parameter. -/
-def LTS.MayTerminate (s : State) : Prop := ∃ s', Terminated s' ∧ lts.CanReach s s'
-
-/-- A state 'is stuck' if it is not terminated and cannot go forward. The definition of `Terminated`
-is a parameter. -/
-def LTS.Stuck (s : State) : Prop :=
-  ¬Terminated s ∧ ¬∃ μ s', lts.Tr s μ s'
-
-end Termination
-
-section Union
-/-! ## Definitions for the unions of LTSs
-
-Note: there is a nontrivial balance between ergonomics and generality here. These definitions might
-change in the future. -/
-
-variable {State : Type u} {Label : Type v}
-
-/-- The union of two LTSs defined on the same types. -/
-def LTS.union (lts1 lts2 : LTS State Label) : LTS State Label where
-  Tr := lts1.Tr ⊔ lts2.Tr
-
-/-- The union of two LTSs that have common supertypes for states and labels. -/
-def LTS.unionSubtype
-{S1 : State → Prop} {L1 : Label → Prop} {S2 : State → Prop} {L2 : Label → Prop}
-[DecidablePred S1] [DecidablePred L1] [DecidablePred S2] [DecidablePred L2]
-(lts1 : LTS (@Subtype State S1) (@Subtype Label L1))
-(lts2 : LTS (@Subtype State S2) (@Subtype Label L2)) :
-  LTS State Label where
-  Tr := fun s μ s' =>
-    if h : S1 s ∧ L1 μ ∧ S1 s' then
-      lts1.Tr ⟨s, h.1⟩ ⟨μ, h.2.1⟩ ⟨s', h.2.2⟩
-    else if h : S2 s ∧ L2 μ ∧ S2 s' then
-      lts2.Tr ⟨s, h.1⟩ ⟨μ, h.2.1⟩ ⟨s', h.2.2⟩
-    else
-      False
-
-/-- Lifting of an `LTS State Label` to `LTS (State ⊕ State') Label`. -/
-def LTS.inl (lts : LTS State Label) :
-    LTS { x : State ⊕ State' // x.isLeft } { _label : Label // True } where
-  Tr s μ s' :=
-    match s, s' with
-    | ⟨.inl s1, _⟩, ⟨.inl s2, _⟩ => lts.Tr s1 μ s2
-    | _, _ => False
-
-/-- Lifting of an `LTS State Label` to `LTS (State' ⊕ State) Label`. -/
-def LTS.inr (lts : LTS State Label) :
-    LTS { x : State' ⊕ State // x.isRight } { _label : Label // True } where
-  Tr s μ s' :=
-    match s, s' with
-    | ⟨.inr s1, _⟩, ⟨.inr s2, _⟩ => lts.Tr s1 μ s2
-    | _, _ => False
-
-/-- Union of two LTSs with the same `Label` type. The result combines the original respective state
-types `State1` and `State2` into `(State1 ⊕ State2)`. -/
-def LTS.unionSum (lts1 : LTS State1 Label) (lts2 : LTS State2 Label) :
-    LTS (State1 ⊕ State2) Label :=
-  LTS.unionSubtype lts1.inl lts2.inr
-
-end Union
 
 section Classes
 /-!
@@ -608,97 +163,97 @@ variable {State : Type u} {Label : Type v} (lts : LTS State Label)
 /-- An lts is deterministic if a state cannot reach different states with the same transition
 label. -/
 @[scoped grind]
-class LTS.Deterministic (lts : LTS State Label) where
+class Deterministic (lts : LTS State Label) where
   deterministic (s1 : State) (μ : Label) (s2 s3 : State) :
     lts.Tr s1 μ s2 → lts.Tr s1 μ s3 → s2 = s3
 
 /-- The `μ`-image of a state `s` is the set of all `μ`-derivatives of `s`. -/
 @[scoped grind =]
-def LTS.image (s : State) (μ : Label) : Set State := { s' : State | lts.Tr s μ s' }
+def image (s : State) (μ : Label) : Set State := { s' : State | lts.Tr s μ s' }
 
 /-- The `μs`-image of a state `s`, where `μs` is a list of labels, is the set of all
 `μs`-derivatives of `s`. -/
 @[scoped grind =]
-def LTS.imageMultistep (s : State) (μs : List Label) : Set State :=
+def imageMultistep (s : State) (μs : List Label) : Set State :=
   { s' : State | lts.MTr s μs s' }
 
 /-- The `μ`-image of a set of states `S` is the union of all `μ`-images of the states in `S`. -/
 @[scoped grind =]
-def LTS.setImage (S : Set State) (μ : Label) : Set State :=
+def setImage (S : Set State) (μ : Label) : Set State :=
   ⋃ s ∈ S, lts.image s μ
 
 /-- The `μs`-image of a set of states `S`, where `μs` is a list of labels, is the union of all
 `μs`-images of the states in `S`. -/
 @[scoped grind =]
-def LTS.setImageMultistep (S : Set State) (μs : List Label) : Set State :=
+def setImageMultistep (S : Set State) (μs : List Label) : Set State :=
   ⋃ s ∈ S, lts.imageMultistep s μs
 
 /-- Characterisation of `setImage` wrt `Tr`. -/
 @[scoped grind =]
-theorem LTS.mem_setImage {lts : LTS State Label} :
+theorem mem_setImage {lts : LTS State Label} :
   s' ∈ lts.setImage S μ ↔ ∃ s ∈ S, lts.Tr s μ s' := by
   simp only [setImage, Set.mem_iUnion, exists_prop]
   grind
 
-theorem LTS.tr_setImage {lts : LTS State Label} (hs : s ∈ S) (htr : lts.Tr s μ s') :
+theorem tr_setImage {lts : LTS State Label} (hs : s ∈ S) (htr : lts.Tr s μ s') :
   s' ∈ lts.setImage S μ := by grind
 
 /-- Characterisation of `setImageMultistep` with `MTr`. -/
 @[scoped grind =]
-theorem LTS.mem_setImageMultistep {lts : LTS State Label} :
+theorem mem_setImageMultistep {lts : LTS State Label} :
   s' ∈ lts.setImageMultistep S μs ↔ ∃ s ∈ S, lts.MTr s μs s' := by
   simp only [setImageMultistep, Set.mem_iUnion, exists_prop]
   grind
 
 @[scoped grind <=]
-theorem LTS.mTr_setImage {lts : LTS State Label} (hs : s ∈ S) (htr : lts.MTr s μs s') :
+theorem mTr_setImage {lts : LTS State Label} (hs : s ∈ S) (htr : lts.MTr s μs s') :
   s' ∈ lts.setImageMultistep S μs := by grind
 
 /-- The image of the empty set is always the empty set. -/
 @[scoped grind =]
-theorem LTS.setImage_empty (lts : LTS State Label) : lts.setImage ∅ μ = ∅ := by grind
+theorem setImage_empty (lts : LTS State Label) : lts.setImage ∅ μ = ∅ := by grind
 
 @[scoped grind =]
-lemma LTS.setImageMultistep_setImage_head (lts : LTS State Label) :
+lemma setImageMultistep_setImage_head (lts : LTS State Label) :
   lts.setImageMultistep S (μ :: μs) = lts.setImageMultistep (lts.setImage S μ ) μs := by grind
 
-/-- Characterisation of `LTS.setImageMultistep` as `List.foldl` on `LTS.setImage`. -/
+/-- Characterisation of `setImageMultistep` as `List.foldl` on `setImage`. -/
 @[scoped grind _=_]
-theorem LTS.setImageMultistep_foldl_setImage (lts : LTS State Label) :
+theorem setImageMultistep_foldl_setImage (lts : LTS State Label) :
   lts.setImageMultistep = List.foldl lts.setImage := by
   ext S μs s'
   induction μs generalizing S <;> grind
 
 /-- Characterisation of membership in `List.foldl lts.setImage` with `MTr`. -/
 @[scoped grind =]
-theorem LTS.mem_foldl_setImage (lts : LTS State Label) :
+theorem mem_foldl_setImage (lts : LTS State Label) :
   s' ∈ List.foldl lts.setImage S μs ↔ ∃ s ∈ S, lts.MTr s μs s' := by
-  rw [← LTS.setImageMultistep_foldl_setImage]
-  exact LTS.mem_setImageMultistep
+  rw [← setImageMultistep_foldl_setImage]
+  exact mem_setImageMultistep
 
 /-- An lts is image-finite if all images of its states are finite. -/
-abbrev LTS.ImageFinite := ∀ s μ, Finite (lts.image s μ)
+abbrev ImageFinite := ∀ s μ, Finite (lts.image s μ)
 
 /-- In a deterministic LTS, if a state has a `μ`-derivative, then it can have no other
 `μ`-derivative. -/
 @[scoped grind .]
-theorem LTS.deterministic_not_lto [h : lts.Deterministic] :
+theorem deterministic_not_lto [h : lts.Deterministic] :
   ∀ s μ s' s'', s' ≠ s'' → lts.Tr s μ s' → ¬lts.Tr s μ s'' := by grind
 
 @[scoped grind _=_]
-theorem LTS.deterministic_tr_image_singleton [lts.Deterministic] :
+theorem deterministic_tr_image_singleton [lts.Deterministic] :
     lts.image s μ = {s'} ↔ lts.Tr s μ s' := by
   have := (lts.image s μ).eq_singleton_iff_unique_mem (a := s')
   grind
 
 /-- In a deterministic LTS, any image is either a singleton or the empty set. -/
 @[scoped grind .]
-theorem LTS.deterministic_image_char [lts.Deterministic] (s : State) (μ : Label) :
+theorem deterministic_image_char [lts.Deterministic] (s : State) (μ : Label) :
     (∃ s', lts.image s μ = { s' }) ∨ (lts.image s μ = ∅) := by grind
 
 /-- In a deterministic LTS, the image of any state-label combination is finite. -/
 instance [lts.Deterministic] (s : State) (μ : Label) : Finite (lts.image s μ) := by
-  have hDet := LTS.deterministic_image_char lts s μ
+  have hDet := deterministic_image_char lts s μ
   cases hDet
   case inl hDet =>
     obtain ⟨s', hDet'⟩ := hDet
@@ -709,276 +264,42 @@ instance [lts.Deterministic] (s : State) (μ : Label) : Finite (lts.image s μ) 
     apply Set.finite_empty
 
 /-- Every deterministic LTS is also image-finite. -/
-instance LTS.deterministic_imageFinite [lts.Deterministic] : lts.ImageFinite := inferInstance
+instance deterministic_imageFinite [lts.Deterministic] : lts.ImageFinite := inferInstance
 
 /-- Every finite-state LTS is also image-finite. -/
 @[scoped grind .]
-instance LTS.finiteState_imageFinite [Finite State] : lts.ImageFinite := inferInstance
+instance finiteState_imageFinite [Finite State] : lts.ImageFinite := inferInstance
 
 /-- A state has an outgoing label `μ` if it has a `μ`-derivative. -/
-def LTS.HasOutLabel (s : State) (μ : Label) : Prop :=
+def HasOutLabel (s : State) (μ : Label) : Prop :=
   ∃ s', lts.Tr s μ s'
 
 /-- The set of outgoing labels of a state. -/
-def LTS.outgoingLabels (s : State) := { μ | lts.HasOutLabel s μ }
+def outgoingLabels (s : State) := { μ | lts.HasOutLabel s μ }
 
 /-- An LTS is finitely branching if it is image-finite and all states have finite sets of
 outgoing labels. -/
-class LTS.FinitelyBranching where
+class FinitelyBranching where
   [image_finite : lts.ImageFinite]
   [finite_state : ∀ s, Finite (lts.outgoingLabels s)]
 
-attribute [instance] LTS.FinitelyBranching.image_finite LTS.FinitelyBranching.finite_state
+attribute [instance] FinitelyBranching.image_finite FinitelyBranching.finite_state
 
 /-- Every LTS with finite types for states and labels is also finitely branching. -/
-instance LTS.FinitelyBranching.of_finite [Finite State] [Finite Label] : lts.FinitelyBranching where
+instance FinitelyBranching.of_finite [Finite State] [Finite Label] : lts.FinitelyBranching where
 
 /-- An LTS is acyclic if there are no infinite multistep transitions. -/
-class LTS.Acyclic (lts : LTS State Label) where
+class Acyclic (lts : LTS State Label) where
   acyclic : ∃ n, ∀ s1 μs s2, lts.MTr s1 μs s2 → μs.length < n
 
 /-- An LTS is finite if it is finite-state and acyclic.
 
 We call this `FiniteLTS` instead of just `Finite` to avoid confusion with the standard `Finite`
 class. -/
-class LTS.FiniteLTS [Finite State] (lts : LTS State Label) extends lts.Acyclic
+class FiniteLTS [Finite State] (lts : LTS State Label) extends lts.Acyclic
 
 end Classes
 
-/-! ## Weak transitions (single- and multistep) -/
-
-section Weak
-
-/-- A type of transition labels that includes a special 'internal' transition `τ`. -/
-class HasTau (Label : Type v) where
-  /-- The internal transition label, also known as τ. -/
-  τ : Label
-
-/-- Saturated τ-transition relation. -/
-def LTS.τSTr [HasTau Label] (lts : LTS State Label) : State → State → Prop :=
-  Relation.ReflTransGen (Tr.toRelation lts HasTau.τ)
-
-/-- Saturated transition relation. -/
-inductive LTS.STr [HasTau Label] (lts : LTS State Label) : State → Label → State → Prop where
-| refl : lts.STr s HasTau.τ s
-| tr : lts.τSTr s1 s2 → lts.Tr s2 μ s3 → lts.τSTr s3 s4 → lts.STr s1 μ s4
-
-/-- The `LTS` obtained by saturating the transition relation in `lts`. -/
-@[scoped grind =]
-def LTS.saturate [HasTau Label] (lts : LTS State Label) : LTS State Label where
-  Tr := lts.STr
-
-@[scoped grind _=_]
-theorem LTS.saturate_tr_sTr [HasTau Label] {lts : LTS State Label} :
-  lts.saturate.Tr = lts.STr := by rfl
-
-/-- Any transition is also a saturated transition. -/
-theorem LTS.STr.single [HasTau Label] (lts : LTS State Label) :
-    lts.Tr s μ s' → lts.STr s μ s' := by
-  intro h
-  apply LTS.STr.tr .refl h .refl
-
-/-- STr transitions labeled by HasTau.τ are exactly the τSTr transitions. -/
-theorem LTS.sTr_τSTr [HasTau Label] (lts : LTS State Label) :
-  lts.STr s HasTau.τ s' ↔ lts.τSTr s s' := by
-  apply Iff.intro <;> intro h
-  case mp =>
-    cases h
-    case refl => exact .refl
-    case tr _ _ h1 h2 h3 =>
-      exact (.trans h1 (.head h2 h3))
-  case mpr =>
-    cases h
-    case refl => exact LTS.STr.refl
-    case tail _ h1 h2 => exact LTS.STr.tr h1 h2 .refl
-
-/-- In a saturated LTS, the transition and saturated transition relations are the same. -/
-theorem LTS.saturate_τSTr_τSTr [hHasTau : HasTau Label] (lts : LTS State Label)
-  : lts.saturate.τSTr s = lts.τSTr s := by
-  ext s''
-  apply Iff.intro <;> intro h
-  case mp =>
-    induction h
-    case refl => constructor
-    case tail _ _ _ h2 h3 => exact Relation.ReflTransGen.trans h3 ((LTS.sTr_τSTr _).mp h2)
-  case mpr =>
-    cases h
-    case refl => constructor
-    case tail s' h2 h3 =>
-      have h4 := LTS.STr.tr h2 h3 Relation.ReflTransGen.refl
-      exact Relation.ReflTransGen.single h4
-
-/-- Saturated transitions labelled by τ can be composed. -/
-@[scoped grind .]
-theorem LTS.STr.trans_τ
-  [HasTau Label] (lts : LTS State Label)
-  (h1 : lts.STr s1 HasTau.τ s2) (h2 : lts.STr s2 HasTau.τ s3) :
-  lts.STr s1 HasTau.τ s3 := by
-  rw [LTS.sTr_τSTr _] at h1 h2
-  rw [LTS.sTr_τSTr _]
-  apply Relation.ReflTransGen.trans h1 h2
-
-/-- Saturated transitions can be composed. -/
-theorem LTS.STr.comp
-  [HasTau Label] (lts : LTS State Label)
-  (h1 : lts.STr s1 HasTau.τ s2)
-  (h2 : lts.STr s2 μ s3)
-  (h3 : lts.STr s3 HasTau.τ s4) :
-  lts.STr s1 μ s4 := by
-  rw [LTS.sTr_τSTr _] at h1 h3
-  cases h2
-  case refl =>
-    rw [LTS.sTr_τSTr _]
-    apply Relation.ReflTransGen.trans h1 h3
-  case tr _ _ hτ1 htr hτ2 =>
-    exact LTS.STr.tr (Relation.ReflTransGen.trans h1 hτ1) htr (Relation.ReflTransGen.trans hτ2 h3)
-
-/-- In a saturated LTS, the transition and saturated transition relations are the same. -/
-theorem LTS.saturate_tr_saturate_sTr [hHasTau : HasTau Label] (lts : LTS State Label)
-  (hμ : μ = hHasTau.τ) : lts.saturate.Tr s μ = lts.saturate.STr s μ := by
-  ext s'
-  apply Iff.intro <;> intro h
-  case mp =>
-    cases h
-    case refl => constructor
-    case tr hstr1 htr hstr2 =>
-      apply LTS.STr.single
-      exact LTS.STr.tr hstr1 htr hstr2
-  case mpr =>
-    cases h
-    case refl => constructor
-    case tr hstr1 htr hstr2 =>
-      rw [LTS.saturate_τSTr_τSTr lts] at hstr1 hstr2
-      rw [←LTS.sTr_τSTr lts] at hstr1 hstr2
-      exact LTS.STr.comp lts hstr1 htr hstr2
-
-/-- In a saturated LTS, every state is in its τ-image. -/
-@[scoped grind .]
-theorem LTS.mem_saturate_image_τ [HasTau Label] (lts : LTS State Label) :
-  s ∈ lts.saturate.image s HasTau.τ := LTS.STr.refl
-
-/-- The `τ`-closure of a set of states `S` is the set of states reachable by any state in `S`
-by performing only `τ`-transitions. -/
-def LTS.τClosure [HasTau Label] (lts : LTS State Label) (S : Set State) : Set State :=
-  lts.saturate.setImage S HasTau.τ
-
-end Weak
-
-/-! ## Divergence -/
-
-section Divergence
-
-/-- An infinite trace is divergent if every label within it is τ. -/
-def LTS.DivergentTrace [HasTau Label] (μs : ωSequence Label) := ∀ i, μs i = HasTau.τ
-
-/-- A state is divergent if there is a divergent execution from it. -/
-def LTS.Divergent [HasTau Label] (lts : LTS State Label) (s : State) : Prop :=
-  ∃ ss μs, lts.OmegaExecution ss μs ∧ ss 0 = s ∧ DivergentTrace μs
-
-/-- If a trace is divergent, then any 'suffix' is also divergent. -/
-@[scoped grind ⇒]
-theorem LTS.divergentTrace_drop
-    [HasTau Label] {μs : ωSequence Label}
-    (h : DivergentTrace μs) (n : ℕ) :
-    DivergentTrace (μs.drop n) := by
-  intro m
-  simp only [DivergentTrace] at h
-  simp only [ωSequence.get_fun, ωSequence.drop]
-  grind
-
-/-- An LTS is divergence-free if it has no divergent state. -/
-class LTS.DivergenceFree [HasTau Label] (lts : LTS State Label) where
-  divergence_free : ¬∃ s, lts.Divergent s
-
-end Divergence
-
-meta section
-
-open Lean Elab Meta Command Term
-
-/-- A command to create an `LTS` from a labelled transition `α → β → α → Prop`, robust to use of
-`variable `-/
-elab "create_lts" lt:ident name:ident : command => do
-  liftTermElabM do
-    let lt ← realizeGlobalConstNoOverloadWithInfo lt
-    let (declName, _) ← mkDeclName (← getCurrNamespace) default name.getId
-    let ci ← getConstInfo lt
-    forallTelescope ci.type fun args ty => do
-      let throwNotLT := throwError m!"type{indentExpr ci.type}\nis not a labelled transition"
-      unless args.size ≥ 2 do
-        throwNotLT
-      unless ← isDefEq (← inferType args[args.size - 3]!) (← inferType args[args.size - 1]!) do
-        throwNotLT
-      unless (← whnf ty).isProp do
-        throwError m!"expecting Prop, not{indentExpr ty}"
-      let params := ci.levelParams.map .param
-      let lt := mkAppN (.const lt params) args[0:args.size-3]
-      let bundle ← mkAppM ``LTS.mk #[lt]
-      let value ← mkLambdaFVars args[0:args.size-3] bundle
-      let type ← inferType value
-      addAndCompile <| .defnDecl {
-        name := declName
-        levelParams := ci.levelParams
-        type
-        value
-        safety := .safe
-        hints := Lean.ReducibilityHints.abbrev
-      }
-      addTermInfo' name (.const declName params) (isBinder := true)
-      addDeclarationRangesFromSyntax declName name
-
-/--
-  This command adds transition notations for an `LTS`. This should not usually be called directly,
-  but from the `lts` attribute.
-
-  As an example `lts_transition_notation foo "β"` will add the notations "[⬝]⭢β" and "[⬝]↠β"
-
-  Note that the string used will afterwards be registered as a notation. This means that if you have
-  also used this as a constructor name, you will need quotes to access corresponding cases, e.g. «β»
-  in the above example.
--/
-syntax attrKind "lts_transition_notation" ident (str)? : command
-macro_rules
-  | `($kind:attrKind lts_transition_notation $lts $sym) =>
-    `(
-      @[nolint docBlame]
-      $kind:attrKind notation3 t:39 "["μ"]⭢" $sym:str t':39 => (LTS.Tr.toRelation $lts μ) t t'
-      @[nolint docBlame]
-      $kind:attrKind notation3 t:39 "["μs"]↠" $sym:str t':39 => (LTS.MTr.toRelation $lts μs) t t'
-     )
-  | `($kind:attrKind lts_transition_notation $lts) =>
-    `(
-      @[nolint docBlame]
-      $kind:attrKind notation3 t:39 "["μ"]⭢" t':39 => (LTS.Tr.toRelation $lts μ) t t'
-      @[nolint docBlame]
-      $kind:attrKind notation3 t:39 "["μs"]↠" t':39 => (LTS.MTr.toRelation $lts μs) t t'
-     )
-
-/-- This attribute calls the `lts_transition_notation` command for the annotated declaration. -/
-syntax (name := lts_attr) "lts" ident (ppSpace str)? : attr
-
-initialize Lean.registerBuiltinAttribute {
-  name := `lts_attr
-  descr := "Register notation for an LTS"
-  add := fun decl stx _ => MetaM.run' do
-    let currNamespace ← getCurrNamespace
-    match stx with
-    | `(attr | lts $lts $sym) =>
-        let mut sym := sym
-        unless sym.getString.endsWith " " do
-          sym := Syntax.mkStrLit (sym.getString ++ " ")
-        liftCommandElabM <| do
-          modifyScope ({ · with currNamespace })
-          Command.elabCommand (← `(create_lts $(mkIdent decl) $lts))
-          Command.elabCommand (← `(scoped lts_transition_notation $lts $sym))
-    | `(attr | lts $lts) =>
-        liftCommandElabM <| do
-          modifyScope ({ · with currNamespace })
-          Command.elabCommand (← `(create_lts $(mkIdent decl) $lts))
-          Command.elabCommand (← `(scoped lts_transition_notation $lts))
-    | _ => throwError "invalid syntax for 'lts' attribute"
-}
-
-end
+end LTS
 
 end Cslib
