CslibTests/HML.lean
@@ -10,7 +10,7 @@ import Cslib.Languages.CCS.Semantics
 namespace CslibTests
 
 open Cslib
-open CCS Logic.HML
+open CCS Logic.HML LTS
 
 example [∀ p μ, Finite ((CCS.lts (defs := defs)).image p μ)] :
     TheoryEq (CCS.lts (defs := defs)) = Bisimilarity (CCS.lts (defs := defs)) :=
